examples/llist.v
@@ -1,3 +1,15 @@
+(*
+Copyright 2010 IMDEA Software Institute
+Licensed under the Apache License, Version 2.0 (the "License");
+you may not use this file except in compliance with the License.
+You may obtain a copy of the License at
+    http://www.apache.org/licenses/LICENSE-2.0
+Unless required by applicable law or agreed to in writing, software
+distributed under the License is distributed on an "AS IS" BASIS,
+WITHOUT WARRANTIES OR CONDITIONS OF ANY KIND, either express or implied.
+See the License for the specific language governing permissions and
+limitations under the License.
+*)
 
 From mathcomp Require Import ssreflect ssrbool ssrnat eqtype ssrfun seq.
 From pcm Require Import options axioms pred.
@@ -11,7 +23,7 @@ From htt Require Import options model heapauto.
 Fixpoint lseg {A} (p q : ptr) (xs : seq A) :=
   if xs is hd::tl then
     [Pred h | exists r h',
-       h = p :-> hd \+ (p .+ 1 :-> r \+ h') /\ h' \In lseg r q tl]
+       h = p :-> hd \+ (p.+1 :-> r \+ h') /\ h' \In lseg r q tl]
   else [Pred h | p = q /\ h = Unit].
 
 Definition EmptyList : exn := exn_from_nat 15.
@@ -23,22 +35,24 @@ Variable A : Type.
 
 Lemma lseg_rcons (xs : seq A) x p r h :
         h \In lseg p r (rcons xs x) <->
-        exists q h', h = h' \+ (q :-> x \+ q .+ 1 :-> r) /\ h' \In lseg p q xs.
+        exists q h', h = h' \+ (q :-> x \+ q.+1 :-> r) /\ 
+                     h' \In lseg p q xs.
 Proof.
 move: xs x p r h; elim=>[|x xs IH] y p r h /=.
 - by split; case=>x [h'][->][<- ->]; [exists p | exists r]; hhauto.
 split.
 - case=>z [h1][->]; case/IH=>w [h2][->] H1.
-  by exists w, (p :-> x \+ (p .+ 1 :-> z \+ h2)); hhauto.
+  by exists w, (p :-> x \+ (p.+1 :-> z \+ h2)); hhauto.
 case=>q [h1][->][z][h2][->] H1.
-exists z, (h2 \+ q :-> y \+ q .+ 1 :-> r).
+exists z, (h2 \+ q :-> y \+ q.+1 :-> r).
 by rewrite -!joinA; split=>//; apply/IH; eauto.
 Qed.
 
 (* null pointer represents an empty segment *)
 
 Lemma lseg_null (xs : seq A) q h :
-        valid h -> h \In lseg null q xs ->
+        valid h -> 
+        h \In lseg null q xs ->
         [/\ q = null, xs = [::] & h = Unit].
 Proof.
 case: xs=>[|x xs] D /= H; first by case: H=><- ->.
@@ -47,9 +61,11 @@ Qed.
 
 (* empty heap represents an empty segment *)
 
-Lemma lseg_empty (xs : seq A) p q : Unit \In lseg p q xs -> p = q /\ xs = [::].
+Lemma lseg_empty (xs : seq A) p q : 
+        Unit \In lseg p q xs -> 
+        p = q /\ xs = [::].
 Proof.
-by case: xs=>[|x xs][] // r [h][/esym/join0E][/unitbE]; rewrite /heap_pts ptsU um_unitbU.
+by case: xs=>[|x xs][] //= r [h][/esym/umap0E][/unitbP]; rewrite um_unitbU.
 Qed.
 
 (* reformulation of the specification *)
@@ -59,7 +75,7 @@ Lemma lseg_case (xs : seq A) p q h :
         [/\ p = q, xs = [::] & h = Unit] \/
         exists x r h',
           [/\ xs = x :: behead xs,
-              h = p :-> x \+ (p .+ 1 :-> r \+ h') &
+              h = p :-> x \+ (p.+1 :-> r \+ h') &
               h' \In lseg r q (behead xs)].
 Proof.
 case: xs=>[|x xs] /=; first by case=>->->; left.
@@ -72,7 +88,7 @@ Corollary lseg_neq (xs : seq A) p q h :
         p != q -> h \In lseg p q xs ->
         exists x r h',
          [/\ xs = x :: behead xs,
-             h = p :-> x \+ (p .+ 1 :-> r \+ h') &
+             h = p :-> x \+ (p.+1 :-> r \+ h') &
              h' \In lseg r q (behead xs)].
 Proof.
 move=>H /lseg_case; case=>//; case=>E.
@@ -81,11 +97,11 @@ Qed.
 
 (* non-empty list is represented by a non-trivial segment *)
 
-Corollary lseg_lt0n (xs : seq A) p q h :
+Lemma lseg_lt0n (xs : seq A) p q h :
         0 < size xs -> h \In lseg p q xs ->
         exists x r h',
          [/\ xs = x :: behead xs,
-             h = p :-> x \+ (p .+ 1 :-> r \+ h') &
+             h = p :-> x \+ (p.+1 :-> r \+ h') &
              h' \In lseg r q (behead xs)].
 Proof.
 move=>H /lseg_case; case=>//; case=>_ E.
@@ -103,7 +119,7 @@ elim: xs h p=>/=.
   by case=>j[_][h2][{h}-> [->->]]; rewrite unitL.
 move=>x xs IH h p; split.
 - case=>r[_][{h}-> /IH][j][h1][h2][-> H1 H2].
-  exists j, (p :-> x \+ p.+ 1 :-> r \+ h1), h2; rewrite !joinA; split=>//.
+  exists j, (p :-> x \+ p.+1 :-> r \+ h1), h2; rewrite !joinA; split=>//.
   by exists r, h1; rewrite joinA.
 case=>j[_][h2][{h}-> [r][h1][-> H1 H2]].
 exists r, (h1 \+ h2); rewrite !joinA; split=>//.
@@ -121,21 +137,26 @@ Variable (A : Type).
 (* specializing the null and neq lemmas *)
 
 Lemma lseq_null (xs : seq A) h :
-        valid h -> h \In lseq null xs -> xs = [::] /\ h = Unit.
+        valid h -> 
+        h \In lseq null xs -> 
+        xs = [::] /\ h = Unit.
 Proof. by move=>D; case/(lseg_null D)=>_ ->. Qed.
 
 Lemma lseq_pos (xs : seq A) p h :
-        p != null -> h \In lseq p xs ->
+        p != null -> 
+        h \In lseq p xs ->
         exists x r h',
           [/\ xs = x :: behead xs,
-              h = p :-> x \+ (p .+ 1 :-> r \+ h') &
+              h = p :-> x \+ (p.+1 :-> r \+ h') &
               h' \In lseq r (behead xs)].
 Proof. by apply: lseg_neq. Qed.
 
 (* a valid heap cannot match two different specs *)
 
 Lemma lseq_func (l1 l2 : seq A) p h :
-        valid h -> h \In lseq p l1 -> h \In lseq p l2 -> l1 = l2.
+        valid h -> 
+        h \In lseq p l1 -> 
+        h \In lseq p l2 -> l1 = l2.
 Proof.
 elim: l1 l2 p h => [|x1 xt IH] /= l2 p h V.
 - by case=>->->; case/lseq_null.
@@ -156,7 +177,7 @@ Next Obligation. by move=>[] /= _ ->; step. Qed.
 (* prepending a value *)
 
 Program Definition insert p (x : A) :
-  {l}, STsep (lseq p l, [vfun p' => lseq p' (x::l)]) :=
+  STsep {l} (lseq p l, [vfun p' => lseq p' (x::l)]) :=
   Do (q <-- allocb p 2;
       q ::= x;;
       ret q).
@@ -164,14 +185,14 @@ Next Obligation.
 (* pull out ghost var + precondition, run the first step *)
 move=>p x [l][] i /= H; step=>q.
 (* run the last 2 steps, guess the final pointer and heap from the goal *)
-rewrite unitR -joinA; heval.
+by rewrite unitR -joinA; heval.
 Qed.
 
 (* getting the head element *)
 (* an example of a partial program, doesn't modify the heap *)
 
 Program Definition head p :
-  {l}, STsep (lseq p l,
+  STsep {l} (lseq p l,
               fun (y : ans A) h => h \In lseq p l /\
                 match y with Val v => l = v :: behead l
                            | Exn e => e = EmptyList /\ l = [::] end) :=
@@ -193,11 +214,11 @@ Qed.
 (* removing the head element, no-op for an empty list *)
 
 Program Definition remove p :
-  {xs : seq A}, STsep (lseq p xs, [vfun p' => lseq p' (behead xs)]) :=
+  STsep {xs : seq A} (lseq p xs, [vfun p' => lseq p' (behead xs)]) :=
   Do (if p == null then ret p
-      else pnext <-- !(p .+ 1);
+      else pnext <-- !p.+1;
            dealloc p;;
-           dealloc p .+ 1;;
+           dealloc p.+1;;
            ret pnext).
 Next Obligation.
 (* pull out ghost + precondition, branch *)
@@ -215,16 +236,16 @@ Qed.
 (* 1. heap is unchanged *)
 (* 2. total length is accumulator + the length of unprocessed list *)
 Definition lenT : Type := forall (pl : ptr * nat),
-  {xs : seq A}, STsep (lseq pl.1 xs,
+  STsep {xs : seq A} (lseq pl.1 xs,
                       [vfun l h => l == pl.2 + length xs /\ lseq pl.1 xs h]).
 
 Program Definition len p :
-  {xs : seq A}, STsep (lseq p xs,
+  STsep {xs : seq A} (lseq p xs,
                       [vfun l h => l == length xs /\ lseq p xs h]) :=
-  Do (let len := Fix (fun (go : lenT) '(p, l) =>
-                       Do (if p == null then ret l
-                           else pnext <-- !(p .+ 1);
-                                go (pnext, l + 1)))
+  Do (let len := ffix (fun (go : lenT) '(p, l) =>
+                        Do (if p == null then ret l
+                            else pnext <-- !p.+1;
+                                 go (pnext, l + 1)))
       in len (p, 0)).
 (* first, the loop *)
 Next Obligation.
@@ -247,19 +268,19 @@ Qed.
 (* the loop invariant: *)
 (* the first list should not be empty and not overlap the second *)
 Definition catT (p2 : ptr) : Type :=
-  forall (p1 : ptr), {xs1 xs2 : seq A},
-    STsep (fun h => p1 != null /\ (lseq p1 xs1 # lseq p2 xs2) h,
-           [vfun _ : unit => lseq p1 (xs1 ++ xs2)]).
+  forall (p1 : ptr), STsep {xs1 xs2 : seq A}
+    (fun h => p1 != null /\ (lseq p1 xs1 # lseq p2 xs2) h,
+     [vfun _ : unit => lseq p1 (xs1 ++ xs2)]).
 
 Program Definition concat p1 p2 :
-  {xs1 xs2 : seq A}, STsep (lseq p1 xs1 # lseq p2 xs2,
+  STsep {xs1 xs2 : seq A} (lseq p1 xs1 # lseq p2 xs2,
                            [vfun a => lseq a (xs1 ++ xs2)]) :=
-  Do (let cat := Fix (fun (go : catT p2) q =>
-                      Do (next <-- !(q .+ 1);
-                          if (next : ptr) == null
-                             then q .+ 1 ::= p2;;
-                                  ret tt
-                             else go next))
+  Do (let cat := ffix (fun (go : catT p2) q =>
+                       Do (next <-- !q.+1;
+                           if (next : ptr) == null
+                              then q.+1 ::= p2;;
+                                   ret tt
+                              else go next))
       in if p1 == null
            then ret p2
            else cat p1;;
@@ -303,16 +324,16 @@ Qed.
 (* 1. the processed and remaining parts should not overlap *)
 (* 2. the result is processed part + a reversal of remainder *)
 Definition revT : Type := forall (p : ptr * ptr),
-  {i done : seq A}, STsep (lseq p.1 i # lseq p.2 done,
+  STsep {i done : seq A} (lseq p.1 i # lseq p.2 done,
                           [vfun y => lseq y (catrev i done)]).
 
 Program Definition reverse p :
-  {xs : seq A}, STsep (lseq p xs, [vfun p' => lseq p' (rev xs)]) :=
-  Do (let reverse := Fix (fun (go : revT) '(i, done) =>
-                          Do (if i == null then ret done
-                              else next <-- !i .+ 1;
-                                   i .+ 1 ::= done;;
-                                   go (next, i)))
+  STsep {xs : seq A} (lseq p xs, [vfun p' => lseq p' (rev xs)]) :=
+  Do (let reverse := ffix (fun (go : revT) '(i, done) =>
+                           Do (if i == null then ret done
+                               else next <-- !i.+1;
+                                    i.+1 ::= done;;
+                                    go (next, i)))
       in reverse (p, null)).
 (* first, the loop *)
 Next Obligation.
@@ -341,16 +362,16 @@ Variable B : Type.
 (* the result is a mapped list *)
 Definition lmapT (f : A -> B) :=
   forall (p : ptr),
-    {xs : seq A}, STsep (lseq p xs,
+    STsep {xs : seq A} (lseq p xs,
                         [vfun _ : unit => lseq p (map f xs)]).
 
 Program Definition lmap f : lmapT f :=
-  Fix (fun (lmap : lmapT f) p =>
+  ffix (fun (lmap : lmapT f) p =>
     Do (if p == null
         then ret tt
         else t <-- !p;
              p ::= f t;;
-             nxt <-- !p .+ 1;
+             nxt <-- !p.+1;
              lmap nxt)).
 Next Obligation.
 (* pull out ghost + precondition, branch *)
@@ -365,5 +386,5 @@ Qed.
 
 End LList.
 
-Arguments head {A} p.
-Arguments remove {A} p.
+Arguments head {A}.
+Arguments remove {A}.
